Unpack state

src/MicroSail/SemiConcrete/Mutator.v
@@ -503,54 +503,78 @@ Module SemiConcrete
 
   Section SemiConcreteWP.
 
-    Definition scmut_wp {Γ1 Γ2 A}
-      (m : SCMut Γ1 Γ2 A)
-      (POST : A -> SCState Γ2 -> Prop)
-      (s1 : SCState Γ1) : Prop :=
-      outcome_satisfy (m s1) (fun r => POST (scmutres_value r) (scmutres_state r)).
+    Definition SCProp (Γ : PCtx) : Type :=
+      LocalStore Γ -> SCHeap -> Prop.
 
-    Lemma scmut_wp_monotonic {A} {Γ1 Γ2} (m : SCMut Γ1 Γ2 A) (s1 : SCState Γ1)
-      (P Q : A -> SCState Γ2 -> Prop) (PQ : forall a s, P a s -> Q a s) :
-      scmut_wp m P s1 -> scmut_wp m Q s1.
-    Proof. unfold scmut_wp. apply outcome_satisfy_monotonic; intros []; apply PQ. Qed.
+    Definition scmut_wp {Γ1 Γ2 A} (m : SCMut Γ1 Γ2 A) (POST : A -> SCProp Γ2) : SCProp Γ1 :=
+      fun δ h =>
+        outcome_satisfy
+          (m {| scstate_localstore := δ; scstate_heap := h |})
+          (fun r => POST (scmutres_value r) (scstate_localstore (scmutres_state r)) (scstate_heap (scmutres_state r))).
+    Global Arguments scmut_wp : simpl never.
 
-    Lemma scmut_wp_equiv {A} {Γ1 Γ2} (m : SCMut Γ1 Γ2 A) (s1 : SCState Γ1)
-      (P Q : A -> SCState Γ2 -> Prop) (PQ : forall a s, P a s <-> Q a s) :
-        scmut_wp m P s1 <-> scmut_wp m Q s1.
+    Lemma scmut_wp_monotonic {A} {Γ1 Γ2} (m : SCMut Γ1 Γ2 A)
+      (P Q : A -> SCProp Γ2) (PQ : forall a δ h, P a δ h -> Q a δ h) :
+      forall δ h,
+        scmut_wp m P δ h -> scmut_wp m Q δ h.
+    Proof.
+      unfold scmut_wp. intros ? ?.
+      apply outcome_satisfy_monotonic; intros []; apply PQ.
+    Qed.
+
+    Lemma scmut_wp_equiv {A} {Γ1 Γ2} (m : SCMut Γ1 Γ2 A)
+      (P Q : A -> SCProp Γ2) (PQ : forall a δ h, P a δ h <-> Q a δ h) :
+      forall δ h, scmut_wp m P δ h <-> scmut_wp m Q δ h.
     Proof. split; apply scmut_wp_monotonic; apply PQ. Qed.
 
+    Lemma scmut_wp_porue {A Γ} (a : A) (POST : A -> SCProp Γ) :
+      forall δ h,
+        scmut_wp (scmut_pure a) POST δ h <->
+        POST a δ h.
+    Proof. reflexivity. Qed.
+
     Lemma scmut_wp_bind {Γ1 Γ2 Γ3 A B} (ma : SCMut Γ1 Γ2 A) (f : A -> SCMut Γ2 Γ3 B)
-          (POST : B -> SCState Γ3 -> Prop) :
-      forall s1 : SCState Γ1,
-        scmut_wp (scmut_bind ma f) POST s1 <->
-        scmut_wp ma (fun a => scmut_wp (f a) POST) s1.
+      (POST : B -> SCProp Γ3) :
+      forall δ h,
+        scmut_wp (scmut_bind ma f) POST δ h <->
+        scmut_wp ma (fun a => scmut_wp (f a) POST) δ h.
     Proof.
       unfold SCMut, scmut_bind, scmut_wp in *; cbn; intros.
       now rewrite outcome_satisfy_bind.
     Qed.
 
-    Lemma scmut_wp_demonic {Γ1 Γ2 A B} (sm : B -> SCMut Γ1 Γ2 A) (s__sc : SCState Γ1) (POST : A -> SCState Γ2 -> Prop) :
-      scmut_wp (scmut_demonic sm) POST s__sc <-> forall v, scmut_wp (sm v) POST s__sc.
+    Lemma scmut_wp_demonic {Γ1 Γ2 A B} (sm : B -> SCMut Γ1 Γ2 A) (POST : A -> SCProp Γ2) :
+      forall δ h,
+        scmut_wp (scmut_demonic sm) POST δ h <-> forall v, scmut_wp (sm v) POST δ h.
     Proof. unfold scmut_wp, scmut_demonic; cbn; intuition. Qed.
 
-    Lemma scmut_wp_demonic_binary {Γ1 Γ2 A} (sm1 sm2 : SCMut Γ1 Γ2 A) (s__sc : SCState Γ1) (POST : A -> SCState Γ2 -> Prop) :
-      scmut_wp (scmut_demonic_binary sm1 sm2) POST s__sc <->
-      scmut_wp sm1 POST s__sc /\ scmut_wp sm2 POST s__sc.
+    Lemma scmut_wp_demonic_binary {Γ1 Γ2 A} (sm1 sm2 : SCMut Γ1 Γ2 A) (POST : A -> SCProp Γ2) :
+      forall δ h,
+        scmut_wp (scmut_demonic_binary sm1 sm2) POST δ h <->
+        scmut_wp sm1 POST δ h /\ scmut_wp sm2 POST δ h.
     Proof. unfold scmut_wp, scmut_demonic_binary; cbn; intuition. Qed.
 
-    Lemma scmut_wp_angelic {Γ1 Γ2 A B} (sm : B -> SCMut Γ1 Γ2 A) (s__sc : SCState Γ1) (POST : A -> SCState Γ2 -> Prop) :
-      scmut_wp (scmut_angelic sm) POST s__sc <-> exists v, scmut_wp (sm v) POST s__sc.
+    Lemma scmut_wp_angelic {Γ1 Γ2 A B} (sm : B -> SCMut Γ1 Γ2 A) (POST : A -> SCProp Γ2) :
+      forall δ h,
+        scmut_wp (scmut_angelic sm) POST δ h <-> exists v, scmut_wp (sm v) POST δ h.
     Proof. unfold scmut_wp, scmut_angelic; cbn; intuition. Qed.
 
-    Lemma scmut_wp_angelic_binary {Γ1 Γ2 A} (sm1 sm2 : SCMut Γ1 Γ2 A) (s__sc : SCState Γ1) (POST : A -> SCState Γ2 -> Prop) :
-      scmut_wp (scmut_angelic_binary sm1 sm2) POST s__sc <->
-      scmut_wp sm1 POST s__sc \/ scmut_wp sm2 POST s__sc.
+    Lemma scmut_wp_angelic_binary {Γ1 Γ2 A} (sm1 sm2 : SCMut Γ1 Γ2 A) (POST : A -> SCProp Γ2) :
+      forall δ h,
+        scmut_wp (scmut_angelic_binary sm1 sm2) POST δ h <->
+        scmut_wp sm1 POST δ h \/ scmut_wp sm2 POST δ h.
     Proof. unfold scmut_wp, scmut_angelic_binary; cbn; intuition. Qed.
 
-    Lemma scmut_wp_state {Γ1 Γ2 A} (f : SCState Γ1 -> A * SCState Γ2) (POST : A -> SCState Γ2 -> Prop) :
-      forall (s1 : SCState Γ1),
-        scmut_wp (scmut_state f) POST s1 <-> POST (fst (f s1)) (snd (f s1)).
-    Proof. intros s1. cbn. now destruct (f s1); cbn. Qed.
+    Lemma scmut_wp_state {Γ1 Γ2 A} (f : SCState Γ1 -> A * SCState Γ2) (POST : A -> SCProp Γ2) :
+      forall δ h,
+        scmut_wp (scmut_state f) POST δ h <->
+        match f (MkSCState δ h) with
+        | (a,MkSCState δ' h') => POST a δ' h'
+        end.
+    Proof.
+      unfold scmut_wp, scmut_state. cbn.
+      intros ? ?. now destruct (f _).
+    Qed.
 
   End SemiConcreteWP.
 
@@ -561,19 +585,13 @@ Module SemiConcrete
       fun ι =>
       scmut_produce ι req ;;
       scmut_exec s >>= fun v =>
-      scmut_consume (env_snoc ι (result::τ) v) ens ;;
-      scmut_leakcheck
+      scmut_consume (env_snoc ι (result::τ) v) ens
+      (* scmut_leakcheck *)
     end%mut.
 
-  Definition semiconcrete_outcome_contract {Δ : PCtx} {τ : Ty} (c : SepContract Δ τ) (s : Stm Δ τ) :
-    Outcome unit :=
-      ⨂ ι : SymInstance (sep_contract_logic_variables c) =>
-      let δΔ : LocalStore Δ := inst ι (sep_contract_localstore c) in
-      let mut := scmut_contract c s ι in
-      let out := mut (scstate_initial δΔ) in
-      outcome_map (fun _ => tt) out.
-
   Definition ValidContractSCMut {Δ τ} (c : SepContract Δ τ) (body : Stm Δ τ) : Prop :=
-    outcome_satisfy (semiconcrete_outcome_contract c body) (fun _ => True).
+    forall ι : SymInstance (sep_contract_logic_variables c),
+      let δΔ : LocalStore Δ := inst ι (sep_contract_localstore c) in
+      scmut_wp (scmut_contract c body ι) (fun _ _ _ => True) δΔ nil.
 
 End SemiConcrete.
